move required ec cmm vectors to all req ec cmm

TestVectorsAwsCryptographicMaterialProviders/dafny/TestVectorsAwsCryptographicMaterialProviders/src/VectorsComposition/AllDefaultCmm.dfy
@@ -37,100 +37,6 @@ module {:options "-functionSyntax:4"} AllDefaultCmm {
                              providerId := "aws-raw-vectors-persistent-" + AesKey
                            ))
 
-  function SubSets(ec: map<Types.Utf8Bytes, Types.Utf8Bytes>, keys: seq<Types.Utf8Bytes>)
-    : set<map<Types.Utf8Bytes, Types.Utf8Bytes>>
-    requires keys == SortedSets.ComputeSetToOrderedSequence2(ec.Keys, (a, b) => a < b)
-  {
-    if |ec| == 0 then
-      {map[]}
-    else
-      var subsets := SubSets(ec - {keys[0]}, keys[1..]);
-      subsets
-      + (set
-           s <- subsets
-           ::
-             s + map[keys[0] := ec[keys[0]]])
-  }
-
-  const a := UTF8.Encode("a").value
-  const b := UTF8.Encode("b").value
-  const c := UTF8.Encode("c").value
-
-  // Dafny has trouble with complex operations on maps in Java
-  // by decomposing this outside the set comprehension
-  // the translated Java compiles correctly
-  const rootEncryptionContext := map[a := a, b := b]
-  const encryptionContextsToTest := {rootEncryptionContext}
-  const disjointEncryptionContext := map[a := c, b := c, c := c]
-
-  lemma disjointEncryptionContextCorrect()
-    ensures rootEncryptionContext.Values !! disjointEncryptionContext.Values
-    ensures rootEncryptionContext.Items !! disjointEncryptionContext.Items
-  {}
-
-  const SuccessTestingRequiredEncryptionContextKeysReproducedEncryptionContext :=
-    set
-      encryptionContext <- encryptionContextsToTest,
-      requiredEncryptionContextKeys
-      <- set
-           s <- SubSets(
-                  encryptionContext,
-                  SortedSets.ComputeSetToOrderedSequence2(encryptionContext.Keys, (a, b) => a < b))
-           :: s.Keys,
-      reproducedEncryptionContext
-      <- set
-           s <- SubSets(
-                  encryptionContext,
-                  SortedSets.ComputeSetToOrderedSequence2(encryptionContext.Keys, (a, b) => a < b))
-           | s.Keys * requiredEncryptionContextKeys == requiredEncryptionContextKeys
-           :: s
-      ::
-        TestVectors.PositiveEncryptKeyringVector(
-          name := "Success testing requiredEncryptionContextKeys/reproducedEncryptionContext",
-          commitmentPolicy := AllAlgorithmSuites.GetCompatibleCommitmentPolicy(StaticAlgorithmSuite),
-          algorithmSuite := StaticAlgorithmSuite,
-          encryptDescription := RawAesKeyring,
-          decryptDescription := RawAesKeyring,
-          encryptionContext := encryptionContext,
-          requiredEncryptionContextKeys := Some(SortedSets.ComputeSetToSequence(requiredEncryptionContextKeys)),
-          reproducedEncryptionContext := Some(reproducedEncryptionContext)
-        )
-
-  const FailureBadReproducedEncryptionContext :=
-    set
-      encryptionContext <- encryptionContextsToTest,
-      requiredEncryptionContextKeys
-      <- set
-           s <- SubSets(
-                  encryptionContext,
-                  SortedSets.ComputeSetToOrderedSequence2(encryptionContext.Keys, (a, b) => a < b))
-           :: s.Keys,
-      incorrectEncryptionContext
-      <- set
-           s <- SubSets(
-                  disjointEncryptionContext,
-                  SortedSets.ComputeSetToOrderedSequence2(disjointEncryptionContext.Keys, (a, b) => a < b))
-           | s != map[]
-           :: s,
-      reproducedEncryptionContext
-      <- set
-           s <- SubSets(
-                  encryptionContext,
-                  SortedSets.ComputeSetToOrderedSequence2(encryptionContext.Keys, (a, b) => a < b))
-           :: s + incorrectEncryptionContext
-      ::
-        TestVectors.PositiveEncryptNegativeDecryptKeyringVector(
-          name := "Failure of reproducedEncryptionContext",
-          decryptErrorDescription := "The reproducedEncryptionContext is not correct",
-          commitmentPolicy := AllAlgorithmSuites.GetCompatibleCommitmentPolicy(StaticAlgorithmSuite),
-          algorithmSuite := StaticAlgorithmSuite,
-          encryptDescription := RawAesKeyring,
-          decryptDescription := RawAesKeyring,
-          encryptionContext := encryptionContext,
-          requiredEncryptionContextKeys := Some(SortedSets.ComputeSetToSequence(requiredEncryptionContextKeys)),
-          reproducedEncryptionContext := Some(reproducedEncryptionContext)
-        )
-
   const Tests
   := {}
   + {
@@ -161,7 +67,5 @@ module {:options "-functionSyntax:4"} AllDefaultCmm {
       encryptionContext := map[]
     )
   }
-  + FailureBadReproducedEncryptionContext
-  + SuccessTestingRequiredEncryptionContextKeysReproducedEncryptionContext
 
 }
