TestVectorsAwsCryptographicMaterialProviders/dafny/TestVectorsAwsCryptographicMaterialProviders/src/VectorsComposition/AllRequiredEncryptionContextCmm.dfy
@@ -6,9 +6,111 @@ include "AllAlgorithmSuites.dfy"
 module {:options "-functionSyntax:4"} AllRequiredEncryptionContextCmm {
   import opened Wrappers
   import AllAlgorithmSuites
+  import SortedSets
+  import StandardLibrary
   import TestVectors
   import KeyVectorsTypes = AwsCryptographyMaterialProvidersTestVectorKeysTypes
+  import Types = AwsCryptographyMaterialProvidersTypes
+  import AllDefaultCmm
+  
+  import opened UTF8
 
-  const Tests: set<TestVectors.EncryptTestVector> := {}
+  function SubSets(ec: map<Types.Utf8Bytes, Types.Utf8Bytes>, keys: seq<Types.Utf8Bytes>)
+    : set<map<Types.Utf8Bytes, Types.Utf8Bytes>>
+    requires keys == SortedSets.ComputeSetToOrderedSequence2(ec.Keys, (a, b) => a < b)
+  {
+    if |ec| == 0 then
+      {map[]}
+    else
+      var subsets := SubSets(ec - {keys[0]}, keys[1..]);
+      subsets
+      + (set
+           s <- subsets
+           ::
+             s + map[keys[0] := ec[keys[0]]])
+  }
+
+  const a := UTF8.Encode("a").value
+  const b := UTF8.Encode("b").value
+  const c := UTF8.Encode("c").value
+
+  // Dafny has trouble with complex operations on maps in Java
+  // by decomposing this outside the set comprehension
+  // the translated Java compiles correctly
+  const rootEncryptionContext := map[a := a, b := b]
+  const encryptionContextsToTest := {rootEncryptionContext}
+  const disjointEncryptionContext := map[a := c, b := c, c := c]
+
+  lemma disjointEncryptionContextCorrect()
+    ensures rootEncryptionContext.Values !! disjointEncryptionContext.Values
+    ensures rootEncryptionContext.Items !! disjointEncryptionContext.Items
+  {}
+
+  const SuccessTestingRequiredEncryptionContextKeysReproducedEncryptionContext :=
+    set
+      encryptionContext <- encryptionContextsToTest,
+      requiredEncryptionContextKeys
+      <- set
+           s <- SubSets(
+                  encryptionContext,
+                  SortedSets.ComputeSetToOrderedSequence2(encryptionContext.Keys, (a, b) => a < b))
+           :: s.Keys,
+      reproducedEncryptionContext
+      <- set
+           s <- SubSets(
+                  encryptionContext,
+                  SortedSets.ComputeSetToOrderedSequence2(encryptionContext.Keys, (a, b) => a < b))
+           | s.Keys * requiredEncryptionContextKeys == requiredEncryptionContextKeys
+           :: s
+      ::
+        TestVectors.PositiveEncryptKeyringVector(
+          name := "Success testing requiredEncryptionContextKeys/reproducedEncryptionContext",
+          commitmentPolicy := AllAlgorithmSuites.GetCompatibleCommitmentPolicy(AllDefaultCmm.StaticAlgorithmSuite),
+          algorithmSuite := AllDefaultCmm.StaticAlgorithmSuite,
+          encryptDescription := AllDefaultCmm.RawAesKeyring,
+          decryptDescription := AllDefaultCmm.RawAesKeyring,
+          encryptionContext := encryptionContext,
+          requiredEncryptionContextKeys := Some(SortedSets.ComputeSetToSequence(requiredEncryptionContextKeys)),
+          reproducedEncryptionContext := Some(reproducedEncryptionContext)
+        )
+
+  const FailureBadReproducedEncryptionContext :=
+    set
+      encryptionContext <- encryptionContextsToTest,
+      requiredEncryptionContextKeys
+      <- set
+           s <- SubSets(
+                  encryptionContext,
+                  SortedSets.ComputeSetToOrderedSequence2(encryptionContext.Keys, (a, b) => a < b))
+           :: s.Keys,
+      incorrectEncryptionContext
+      <- set
+           s <- SubSets(
+                  disjointEncryptionContext,
+                  SortedSets.ComputeSetToOrderedSequence2(disjointEncryptionContext.Keys, (a, b) => a < b))
+           | s != map[]
+           :: s,
+      reproducedEncryptionContext
+      <- set
+           s <- SubSets(
+                  encryptionContext,
+                  SortedSets.ComputeSetToOrderedSequence2(encryptionContext.Keys, (a, b) => a < b))
+           :: s + incorrectEncryptionContext
+      ::
+        TestVectors.PositiveEncryptNegativeDecryptKeyringVector(
+          name := "Failure of reproducedEncryptionContext",
+          decryptErrorDescription := "The reproducedEncryptionContext is not correct",
+          commitmentPolicy := AllAlgorithmSuites.GetCompatibleCommitmentPolicy(AllDefaultCmm.StaticAlgorithmSuite),
+          algorithmSuite := AllDefaultCmm.StaticAlgorithmSuite,
+          encryptDescription := AllDefaultCmm.RawAesKeyring,
+          decryptDescription := AllDefaultCmm.RawAesKeyring,
+          encryptionContext := encryptionContext,
+          requiredEncryptionContextKeys := Some(SortedSets.ComputeSetToSequence(requiredEncryptionContextKeys)),
+          reproducedEncryptionContext := Some(reproducedEncryptionContext)
+        )
+  // These are only required encryption context vectors with static aes keyrings
+  const Tests: set<TestVectors.EncryptTestVector> :=
+    SuccessTestingRequiredEncryptionContextKeysReproducedEncryptionContext +
+    FailureBadReproducedEncryptionContext 
 
 }
